{\begin{equation*}
	\begin{split}
		\frac{(-3+1)(2(-3))-((-3)^2-3)(1)}{(-3+1)^2} & = \frac{(-3+1)(2(-3)) - ((-3)^2-3)(1)}{(-2)^2} \\
							     & = \frac{(-2)(-6)-((-3)^2-3)(1)}{(-2)^2} \\
							     & = \frac{(-2)(-6) -(9-3)(1)}{(-2)^2} \\
							     & = \frac{(-2)(-6) -(6)(1)}{4} \\
							     & = \frac{-12-6}{4} \\
							     & = \frac{-18}{4} \\
							     & = \frac{-9}{2}
	\end{split}
\end{equation*} 
\vfill\break}
{The final answer is not correct. In the fifth step, $(-2)(-6)$ should be $12$, not $-12$.}
